code/experimental/ed25519/Ed25519.fsti
@@ -11,7 +11,7 @@ let op_String_Access h b = Hacl.Spec.Endianness.reveal_sbytes (as_seq h b)
 val sign:
   signature:hint8_p{length signature = 64} ->
   secret:hint8_p{length secret = 32} ->
-  msg:hint8_p ->
+  msg:hint8_p{length msg < pow2 32 - 64} ->
   len:UInt32.t{UInt32.v len = length msg} ->
   Stack unit
     (requires (fun h -> live h signature /\ live h msg /\ live h secret))
@@ -23,7 +23,7 @@ val sign:
 val verify:
   public:uint8_p{length public = 32} ->
   msg:uint8_p ->
-  len:UInt32.t{length msg = UInt32.v len} ->
+  len:UInt32.t{length msg = UInt32.v len /\ length msg < pow2 32 - 64} ->
   signature:uint8_p{length signature = 64} ->
   Stack bool
     (requires (fun h -> live h public /\ live h msg /\ live h signature))
