code/experimental/ed25519/Hacl.Impl.SHA512.ModQ.fsti
@@ -25,10 +25,10 @@ val sha512_modq_pre_pre2:
   out:buffer Hacl.UInt64.t{length out = 5} ->
   prefix:buffer Hacl.UInt8.t{length prefix = 32 /\ disjoint prefix out} ->
   prefix2:buffer Hacl.UInt8.t{length prefix2 = 32 /\ disjoint prefix2 out} ->
-  input:buffer Hacl.UInt8.t ->
+  input:buffer Hacl.UInt8.t{disjoint out input} ->
   len  :UInt32.t{UInt32.v len = length input /\ length input < pow2 32 - 64} ->
   Stack unit
-        (requires (fun h0 -> live h0 input /\ live h0 out))
+        (requires (fun h -> live h input /\ live h out /\ live h prefix /\ live h prefix2))
         (ensures  (fun h0 _ h1 -> live h0 input /\ live h1 out /\ modifies_1 out h0 h1 /\
           live h0 prefix /\ live h1 prefix /\ live h0 prefix2 /\ live h1 prefix2 /\
           Hacl.Spec.BignumQ.Eval.eval_q (as_seq h1 out) == Spec.Ed25519.sha512_modq FStar.Seq.(as_seq h0 prefix @| as_seq h0 prefix2 @| as_seq h0 input) /\
