specs/Spec.Chacha20.fst
@@ -33,20 +33,20 @@ let line (a:idx) (b:idx) (d:idx) (s:t{v s < 32}) (m:state) : Tot state =
 let quarter_round a b c d : shuffle = 
   line a b d 16ul @ 
   line c d b 12ul @
-  line a b d 8ul @ 
+  line a b d 8ul  @ 
   line c d b 7ul 
 
 let column_round : shuffle = 
-  quarter_round 0 4 8 12 @
-  quarter_round 1 5 9 13 @
+  quarter_round 0 4 8  12 @
+  quarter_round 1 5 9  13 @
   quarter_round 2 6 10 14 @
   quarter_round 3 7 11 15
 
 let diagonal_round : shuffle = 
   quarter_round 0 5 10 15 @
   quarter_round 1 6 11 12 @
-  quarter_round 2 7 8 13 @
-  quarter_round 3 4 9 14
+  quarter_round 2 7 8  13 @
+  quarter_round 3 4 9  14
 
 let double_round: shuffle = 
     column_round @ diagonal_round (* 2 rounds *)
@@ -71,7 +71,7 @@ let setup (k:key) (n:nonce) (c:counter): Tot state =
   uint32s_from_le 3 n
 
 let chacha20_block (k:key) (n:nonce) (c:counter): Tot block =
-    let st = setup k n c in
+    let st  = setup k n c in
     let st' = chacha20_core st in
     uint32s_to_le 16 st'
 
